compiler/backend/proofs/lab_filterProofScript.sml
@@ -3,6 +3,8 @@ open BasicProvers
 
 val _ = new_theory "lab_filterProof";
 
+val is_Label_def = lab_to_targetTheory.is_Label_def;
+
 val adjust_pc_def = Define `
   adjust_pc p xs =
     if p = 0n then 0n else
